progress

test/TestB.lean
@@ -2,3 +2,7 @@
 def a : Nat := 1
 
 def b : Nat := 1
+
+def c : Nat := 2
+
+def sada : Int := 123
