Leaff/Diff.lean
@@ -9,11 +9,60 @@ import Leaff.HashSet
 # Leaff (Lean Diff) core
 
 ## Main types
+- `Trait` hashable functions of `ConstantInfo`'s used to determine whether two constants are different
 - `Diff` the type of a single human understandable difference between two environments
 
 -/
+open Lean
+/--
+Traits are functions from `ConstantInfo` to some type `α` that when changed,
+results in some meaningful difference between two constants.
+For instance the type, name, value of a constant, or whether it is an axiom,
+theorem, or definition. -/
+structure Trait :=
+  α : Type
+  val : ConstantInfo → α
+  id : Name
+  [ins : Hashable α]
 
-open Lean in
+instance : BEq Trait where
+   beq a b := a.id == b.id
+instance {t : Trait} : Hashable t.α := t.ins
+
+def Trait.mk' (α : Type) [Hashable α] (val : ConstantInfo → α) (name : Name := by exact decl_name%) : Trait := ⟨α, val, name⟩
+namespace Trait
+def type : Trait := Trait.mk' Expr ConstantInfo.type
+def value : Trait := Trait.mk' Expr ConstantInfo.value!
+
+def name : Trait := Trait.mk' Name ConstantInfo.name
+def species : Trait := Trait.mk' String fun
+  | .axiomInfo _ => "axiom"
+  | .defnInfo _ => "def"
+  | .thmInfo _ => "thm"
+  | .opaqueInfo _ => "opaque"
+  | .quotInfo _ => "quot"
+  | .inductInfo _ => "induct"
+  | .ctorInfo _ => "ctor"
+  | .recInfo _ => "rec"
+
+def relevantTraits : List Trait := [name, type, value, species]
+def hashExcept (t : Trait) : ConstantInfo → UInt64 :=
+  (relevantTraits.filter (· != t)).foldl (fun h t c => mixHash (hash (t.val c)) (h c)) (fun _ => 7) -- TODO 0 or 7...
+
+-- section testing
+-- def aaaa := 1
+-- def aaab := 1
+-- #eval show MetaM Unit from do
+--   let e ← getEnv
+--   let n ← e.find? ``aaaa
+--   dbg_trace (hashExcept name n)
+--   let n ← e.find? ``aaab
+--   dbg_trace (hashExcept name n)
+-- end testing
+
+end Trait
+
+open Lean
 /--
 A type representing single differences between two environments, limited
 to changes that a user might wish to see.
@@ -22,10 +71,11 @@ inductive Diff : Type
   | added (name : Name)
   | removed (name : Name)
   | renamed (oldName newName : Name) (namespaceOnly : Bool)
-  | movedToModule (name : Name) -- maybe args here
-  | movedWithinModule (name : Name)
-  | proofChanged (name : Name)
+  | movedToModule (name oldModuleName newModuleName : Name) -- maybe args here
+  | movedWithinModule (name moduleName : Name)
+  | proofChanged (name : Name) (isProofRelevant : Bool) -- TODO maybe value changed also for defs
   | typeChanged (name : Name)
+  | speciesChanged (name : Name) (fro to : String)
   | extensionEntriesModified (ext : Name)
   | docChanged (name : Name) -- TODO how does module/opther doc fit in here
   | docAdded (name : Name)
@@ -40,14 +90,38 @@ inductive Diff : Type
   | transitiveImportRemoved (module importName : Name)
 deriving DecidableEq, Repr
 
+-- TODO changed def to lemma or vice versa
+-- TODO distinguish between proof changed and value changed
 
--- TODO maybe an "optic" for isBlah that returns all args of blah
+
+-- TODO maybe variant "optic"s for isBlah that returns all args of blah not just a bool
 -- set_option trace.derive_optics true
 derive_optics Diff
 
-
-
 namespace Diff
+/-- priority for displaying diffs, lower numbers are more important and should come first in the output -/
+def prio : Diff → Nat
+  | .added _ => 1
+  | .removed _ => 1
+  | .renamed _ _ _ => 2 -- TODO namespace lower
+  | .movedToModule _ _ _ => 2
+  | .movedWithinModule _ _ => 3
+  | .proofChanged _ _ => 2 -- TODO higher if proof relevant
+  | .typeChanged _ => 1
+  | .speciesChanged _ _ _ => 1
+  | .extensionEntriesModified _ => 1
+  | .docChanged _ => 2
+  | .docAdded _ => 2
+  | .docRemoved _ => 1
+  | .moduleRenamed _ _ => 1
+  | .attributeAdded _ _ => 1
+  | .attributeRemoved _ _ => 1
+  | .attributeChanged _ _ => 2
+  | .directImportAdded _ _ => 1
+  | .directImportRemoved _ _ => 2
+  | .transitiveImportAdded _ _ => 3
+  | .transitiveImportRemoved _ _ => 3
+
 open Std
 -- TODO can we make the output richer,
 -- colours
@@ -59,13 +133,30 @@ def summarize (diffs : List Diff) (includeInternals := false) : Format := Id.run
   if diffs = [] then return "No differences found."
   let mut out : Format := ("Found differences:" : Format).append .line
   for d in diffs do
+    -- TODO this should be a match
+    -- TODO should build a big list of types and priorities and then sort by lex on prio then type
+    -- TODO rethink whether internals should be ignored here or in the differ logic
     if d.isAdded   && (includeInternals || !(name! d).isInternal) then out := out.append <| format s!"added {name! d}\n" -- awkward that we can't use dot notation with nested
     if d.isRemoved && (includeInternals || !(name! d).isInternal) then out := out.append <| format s!"removed {name! d}\n"
+    -- TDOO namespaceonly
     if d.isRenamed && (includeInternals || !(oldName! d).isInternal) then out := out.append <| format s!"renamed {oldName! d} → {newName! d}\n"
+    if d.isMovedToModule && (includeInternals || !(name! d).isInternal) then out := out.append <| format s!"moved {name! d} to {newModuleName! d}\n"
+    if d.isMovedWithinModule && (includeInternals || !(name! d).isInternal) then out := out.append <| format s!"moved {name! d} within module {moduleName! d}\n"
+    if d.isProofChanged && (includeInternals || !(name! d).isInternal) then out := out.append <| format s!"proof changed for {name! d}\n"
+    if d.isTypeChanged && (includeInternals || !(name! d).isInternal) then out := out.append <| format s!"type changed for {name! d}\n"
+    if d.isSpeciesChanged && (includeInternals || !(name! d).isInternal) then out := out.append <| format s!"{name! d} changed from {fro! d} to {to! d}\n"
+    if d.isExtensionEntriesModified then out := out.append <| format s!"extension entry modified for {ext! d}\n"
+    if d.isDocChanged then out := out.append <| format s!"doc modified for {name! d}\n"
     if d.isDocAdded   then out := out.append <| format s!"doc added to {name! d}\n"
     if d.isDocRemoved then out := out.append <| format s!"doc removed from {name! d}\n"
-    if d.isDocChanged then out := out.append <| format s!"doc modified for {name! d}\n"
-    if d.isExtensionEntriesModified then out := out.append <| format s!"extension entry modified for {ext! d}\n"
+    if d.isModuleRenamed then out := out.append <| format s!"module renamed {oldName! d} → {newName! d}\n"
+    if d.isAttributeAdded then out := out.append <| format s!"attribute {attrName! d} added to {name! d}\n"
+    if d.isAttributeRemoved then out := out.append <| format s!"attribute {attrName! d} removed from {name! d}\n"
+    if d.isAttributeChanged then out := out.append <| format s!"attribute {attrName! d} changed for {name! d}\n"
+    if d.isDirectImportAdded then out := out.append <| format s!"direct import {importName! d} added to {module! d}\n"
+    if d.isDirectImportRemoved then out := out.append <| format s!"direct import {importName! d} removed from {module! d}\n"
+    if d.isTransitiveImportAdded then out := out.append <| format s!"transitive import {importName! d} added to {module! d}\n"
+    if d.isTransitiveImportRemoved then out := out.append <| format s!"transitive import {importName! d} removed from {module! d}\n"
     -- dbg_trace (repr d)
   out := out.append (format s!"{diffs.length} differences, some not shown")
   pure out
@@ -112,7 +203,11 @@ def extDiffs (old new : Environment) : IO (List Diff) := do
   -- let newexts := RBSet.ofList (new.constants.map₁.toList.map Prod.fst) Name.cmp
   pure out
 
-def diffHash (c : ConstantInfo) : UInt64 := mixHash c.name.hash <| mixHash c.type.hash c.value!.hash
+open Trait
+
+
+-- TODO make this the hash of all relevantTraits, but
+def diffHash (c : ConstantInfo) : UInt64 := mixHash (hash <| species.val c) <| mixHash c.name.hash <| mixHash c.type.hash c.value!.hash
 
 def constantDiffs (old new : Environment) : List Diff := Id.run do
   let mut out : List Diff := []
@@ -122,20 +217,55 @@ def constantDiffs (old new : Environment) : List Diff := Id.run do
   -- TODO should we use rbmap or hashmap?
   -- let oldhashes := (HashMap.fold (fun old name const =>
   --   let ha := (diffHash const)
+  -- let (all, ex) := (HashMap.fold (fun (all, ex) name const =>
+  --   if const.hasValue && ¬ name.isInternal then (all + 1, ex + 1) else (all + 1, ex)) (0,0) old.constants.map₁)
+  -- dbg_trace (all, ex)
   --   old.insert ha <| (old.findD ha #[]).push name) (mkRBMap UInt64 (Array Name) Ord.compare) old.constants.map₁)
+  let sz := max (new.constants.map₁.size / 5) (old.constants.map₁.size / 5)
+
   let oldhashes := (HashMap.fold (fun old name const =>
-    if const.hasValue && ¬ name.isInternal then old.insert name else old) (@HashSet.empty Name _ ⟨fun n => diffHash <| old.constants.map₁.find! n⟩) old.constants.map₁)
+    if const.hasValue && ¬ name.isInternal then old.insert name else old) (@mkHashSet Name _ ⟨fun n => diffHash <| old.constants.map₁.find! n⟩ sz) old.constants.map₁)
   let newhashes := (HashMap.fold (fun old name const =>
-    if const.hasValue && ¬ name.isInternal then old.insert name else old) (@HashSet.empty Name _ ⟨fun n => diffHash <| new.constants.map₁.find! n⟩) new.constants.map₁)
+    if const.hasValue && ¬ name.isInternal then old.insert name else old) (@mkHashSet Name _ ⟨fun n => diffHash <| new.constants.map₁.find! n⟩ sz) new.constants.map₁)
   -- TODO can we fold over smaller
   -- TODO init with right size
   -- out := out ++ (newnames.sdiff oldnames).toList.map .added
   -- out := out ++ (oldnames.sdiff newnames).toList.map .removed
   -- dbg_trace out.length
-  dbg_trace (HashSet.sdiff oldhashes newhashes).toList
-  for (di, removed) in (HashSet.sdiff oldhashes newhashes).toList do
-    if removed then out := .removed di :: out
-    if !removed then out := .added di :: out
+  -- dbg_trace (HashSet.sdiff oldhashes newhashes).toList
+  let diff := (HashSet.sdiff oldhashes newhashes).toList
+  let befores := diff.filterMap (fun (di, bef) => if bef then some (old.constants.map₁.find! di) else none)
+  let afters := diff.filterMap (fun (di, bef) => if bef then none else some (new.constants.map₁.find! di))
+  -- dbg_trace dm.map (fun (c, rem) => (c.name, rem))
+  -- TODO could use hashset here
+  let mut explained := []
+  for t in relevantTraits do
+    let f := t.hashExcept
+    for b in befores do
+      if (b.name, true) ∈ explained then continue
+      for a in afters do
+        if (a.name, false) ∈ explained then continue
+        if f a == f b ∧ t == name then
+          out := .renamed b.name a.name false :: out
+          explained := (a.name, true) :: (b.name, false) :: explained
+          continue
+        if f a == f b ∧ t == value then
+          out := .proofChanged a.name false :: out -- TODO check if proof relevant
+          explained := (a.name, true) :: (b.name, false) :: explained
+          continue
+        if f a == f b ∧ t == type then
+          out := .typeChanged a.name :: out
+          explained := (a.name, true) :: (b.name, false) :: explained
+          continue
+        if f a == f b ∧ t == species then
+          out := .speciesChanged a.name (species.val b) (species.val a) :: out
+          explained := (a.name, true) :: (b.name, false) :: explained
+        -- dbg_trace "asd"
+        -- dbg_trace mat.map ConstantInfo.name
+  for a in afters do
+    if !(a.name, false) ∈ explained then out := .added a.name :: out
+  for b in befores do
+    if !(b.name, true) ∈ explained then out := .removed b.name :: out
   pure out
 
 -- TODO some sort of minimization pass might be needed?
@@ -161,8 +291,9 @@ unsafe
 def summarizeDiffImports (imports₁ imports₂ : Array Import) : IO Unit :=
   diffImports imports₁ imports₂
 
-#eval summarizeDiffImports #[`Std.Lean.Float] #[`Std.Data.Fin.Init.Lemmas]
+#eval summarizeDiffImports #[`Std.Classes.RatCast] #[`Std.Data.Rat]
 -- #eval summarizeDiffImports #[`Mathlib] #[`Std.Data.Fin.Init.Lemmas]
+
 
 #eval summarizeDiffImports #[`test.TestA] #[`test.TestB]
 
