Leaff/HashSet.lean
@@ -1,13 +1,72 @@
 import Lean.Data.HashSet
 import Std.Data.List.Basic
 
+
+namespace Array
+
+
+-- TODO these are copied from lean core but look wrong if stop is too big imo
+
+/-- See comment at `forInUnsafe` -/
+@[inline]
+unsafe def foldlM₂Unsafe {α : Type u} {β : Type v} {m : Type v → Type w} [Monad m] (f : β → α → α → m β) (init : β) (asl asr : Array α) (start := 0) (stop := min asl.size asr.size) : m β :=
+  let rec @[specialize] fold (i : USize) (stop : USize) (b : β) : m β := do
+    if i == stop then
+      pure b
+    else
+      fold (i+1) stop (← f b (asl.uget i lcProof) (asr.uget i lcProof))
+  if start < stop then
+    if stop ≤ min asl.size asr.size then
+      fold (USize.ofNat start) (USize.ofNat stop) init
+    else
+      pure init
+  else
+    pure init
+
+/-- Reference implementation for `foldlM`
+this is a custom fold over a pair of arrays, assuming their sizes are multiples of each other
+-/
+@[implemented_by foldlM₂Unsafe]
+-- todo could be generalized
+def foldlM₂ {α : Type u} {β : Type v} {m : Type v → Type w} [Monad m] (f : β → α → α → m β) (init : β) (asl asr : Array α) (start := 0) (stop := min asl.size asr.size) : m β :=
+  let fold (stop : Nat) (h : stop ≤ min asl.size asr.size) :=
+    let rec loop (i : Nat) (j : Nat) (b : β) : m β := do
+      if hlt : j < stop then
+        match i with
+        | 0    => pure b
+        | i'+1 =>
+          have : j < asl.size := Nat.lt_of_lt_of_le hlt (Nat.le_min.mp h).1
+          have : j < asr.size := Nat.lt_of_lt_of_le hlt (Nat.le_min.mp h).2
+          loop i' (j+1) (← f b asl[j] asr[j])
+      else
+        pure b
+    loop (stop - start) start init
+  if h : stop ≤ min asl.size asr.size then
+    fold stop h
+  else
+    fold (min asl.size asr.size) (Nat.le_refl _)
+
+
+@[inline]
+def foldl₂ {α : Type u} {β : Type v} (f : β → α → α → β) (init : β) (asl asr : Array α) (start := 0) (stop := min asl.size asr.size) : β :=
+  Id.run <| asl.foldlM₂ f init asr start stop
+end Array
+
+
 namespace Lean
+
+@[inline] def HashSetImp.sdiff [BEq α] [Hashable α] (l : HashSetImp α) (r : HashSetImp α) : HashSet (α × Bool) :=
+  -- if l.numBuckets !=
+  --    r.numBuckets then panic! "hash sets have different size" else -- TODO remove this restriction!
+  Array.foldl₂ (fun o ll rl => o.insertMany <| (ll.diff rl).map ((·, true)) ++ (rl.diff ll).map ((·, false))) mkHashSet l.2.1 r.2.1
+
 namespace HashSet
 
 @[inline] def sdiff [BEq α] [Hashable α] (l : @HashSet α _ instl) (r : @HashSet α _ instr) : HashSet (α × Bool) :=
   if l.numBuckets !=
      r.numBuckets then panic! "hash sets have different size" else -- TODO remove this restriction!
-  (l.1.buckets.1.zipWith r.1.buckets.1 fun ll rl => (ll.diff rl).map ((·, true)) ++ (rl.diff ll).map ((·, false))).foldl (fun o li => o.insertMany li) mkHashSet
+  (l.1.sdiff r.1)
+  -- (l.1.buckets.1.zipWith r.1.buckets.1 fun ll rl => (ll.diff rl).map ((·, true)) ++ (rl.diff ll).map ((·, false))).foldl (fun o li => o.insertMany li) mkHashSet
 
 
 #eval (mkHashSet.insertMany [3,4,5,6,7,8,9,0,1,4,6,213,2432,435,435,234,12,2]).numBuckets
