test/TestA.lean
@@ -2,3 +2,7 @@
 
 /-- has a doc -/
 def a : Nat := 1
+
+def c : Nat := 1
+
+theorem sada : Int := 123
